Emit environment to variable morphism directly (#92)
Also mechanize proofs

cava/cava/Cava/Arrow/Syntax/CC.v
@@ -9,41 +9,56 @@ Require Import Cava.Arrow.Syntax.Desugared.
 
 Set Implicit Arguments.
 
+Ltac solver :=
+  simpl in *; try subst; try match goal with
+  | [ H : ?X < ?X |- _ ] => apply Nat.lt_irrefl in H; contradiction
+  | [ H : ?X = ?Y, H1: ?X < ?Y |- _ ] => rewrite H in H1; apply Nat.lt_irrefl in H; contradiction
+
+  | [ |- Some ?X = Some ?X ] => f_equal
+  | [ |- context[eq_nat_dec ?X ?Y] ] => destruct (eq_nat_dec X Y)
+
+  | [ H : None = Some _|- _ ] => inversion H
+  | [ H : Some ?X = Some ?Y |- _ ] => inversion H
+  | [ H : ?X /\ ?Y |- _ ] => inversion H; clear H
+  | [ H : ?X \/ ?Y |- _ \/ ?Y ] => inversion H; [ left; progress eauto | right; progress eauto ]
+  | [ H : ?X \/ ?Y |- _ ] => inversion H; clear H
+
+  | [ H : context[eq_nat_dec ?X ?Y] |- _ ] => destruct (eq_nat_dec X Y)
+  | [ H : ?X = ?Y, H2: ?X = ?Y -> ?Z |- _ ] => apply H2 in H
+
+  | [ H : ?X = ?Y, H2: context[?X] |- _ ] => rewrite H in H2
+
+  | [ H : ?X <> ?X |- _ ] => destruct H
+  end.
+
+Hint Extern 2 => solver : core.
+
+Hint Extern 4 (_ < length (_ :: _)) => simpl : core.
+
 Section WithArrow.
   Variable arr: Arrow.
-
-  (*
-  An environment to track the arrow objects corresponding to variables.
-  Variables are then instantiated as a morphism from the environment to the
-  associated object.
-  *)
-  Inductive environment : nat -> Type :=
-  | ECons : forall n (o: object), environment n -> environment (S n)
-  | ENil : environment 0.
 
   (****************************************************************************)
   (* Environment manipulation                                                 *)
   (****************************************************************************)
 
-  Fixpoint environment_as_object {n} (env: environment n): object :=
+  (* An environment to track the arrow objects corresponding to variables.
+  Variables are then instantiated as a morphism from the environment to the
+  associated object. *)
+  Inductive environment : nat -> Type :=
+  | ECons : forall n (o: object), environment n -> environment (S n)
+  | ENil : environment 0.
+
+  Fixpoint as_object {n} (env: environment n): object :=
   match env with
   | ENil => unit
-  | ECons o env' => o ** environment_as_object env'
+  | ECons o env' => o ** as_object env'
   end.
 
-  Fixpoint environment_objects_as_list {n} (env: environment n): list object :=
+  Fixpoint as_object_list {n} (env: environment n): list object :=
   match env with
   | ENil => []
-  | ECons o env' => o :: environment_objects_as_list env'
-  end.
-
-  (* Creates a right imbalanced tree of hetrogenous morphisms. Morphism
-  * instances can then be recovered from the structure with the help of the
-  * functions below *)
-  Fixpoint env_morphisms (env_obj: object) (env_objs: list object): Type :=
-  match env_objs with
-  | [] => Datatypes.unit
-  | ty::tys => prod (morphism env_obj ty) (env_morphisms env_obj tys)
+  | ECons o env' => o :: as_object_list env'
   end.
 
   Fixpoint lookup_object (n: nat) (env: list object): option object :=
@@ -55,13 +70,9 @@ Section WithArrow.
     else lookup_object n os
   end.
 
-  (* Shorthand for passing evidence that a lookup is well formed *)
-  Notation ok_lookup := (
-    fun (n: nat) (env: list object) (o: object) => lookup_object n env = Some o
-  ).
-
-  (* The type of a morphism in our environment is a morphism from our environment to the
-  * object type at the index n, i.e. env_obj ~> o, where lookup_object n = Some o *)
+  (* The type of an arrow morphism from our environment to a variable is 
+  `as_object env ~> o`
+  where lookup_object n env = Some o *)
   Fixpoint lookup_morphism_ty (n: nat) (env_obj: object) (objs: list object): Type :=
   match objs with
   | [] => Datatypes.unit
@@ -71,177 +82,120 @@ Section WithArrow.
     else lookup_morphism_ty n env_obj os
   end.
 
-  (* Now we have the morphism type, we can pull a morphism out of the
-  * hetrogenous env_obj which contains all the morphisms. *)
-  Definition lookup_morphism (env_obj: object) (objs: list object):
-    forall (n: nat), env_morphisms env_obj objs -> lookup_morphism_ty n env_obj objs.
-  Proof.
-    induction objs;
-    intros.
-
-    - exact tt.
-
-    - simpl.
-      destruct (eq_nat_dec n (length objs)).
-      * exact (fst X).
-
-      * apply IHobjs.
-        exact (snd X).
-  Defined.
-
-  (* Proof that looking up a morphism is the morphism from the environment to
-    * the object at the same index.
-    *)
-  Theorem ok_lookup_sets_lookup_morphism_ty : forall n o objs env_obj,
-    lookup_object n objs = Some o
-    -> lookup_morphism_ty n env_obj objs = morphism env_obj o.
-  Proof.
-    induction objs;
-    intros.
-
-    - simpl in H. easy.
-
-    - simpl in *.
-      destruct (eq_nat_dec n (length objs)); inversion H; auto.
-  Defined.
-
-  Definition morphism_coerce:
-    forall (n:nat) env_obj o (objs: list object),
-    ok_lookup n objs o ->
-    lookup_morphism_ty n env_obj objs -> morphism env_obj o.
-  Proof.
-    intros.
-    apply ok_lookup_sets_lookup_morphism_ty with (env_obj:=env_obj) in H.
-    rewrite H in X.
-    apply X.
-  Defined.
-
-  (* Map over the environment object. This is split into two functions to ease typing as
-  prefixing the existing morphisms means they are not equal to recreating the
-  morphism from the 'environment' they were created with, as the env_obj now
-  contains 'ECons' levels from above. *)
-  Definition contravariant_map'
-    (env_obj env_obj': object)
-    (objs: list object)
-    (map: env_morphisms env_obj objs -> env_morphisms env_obj' objs)
-    (f: env_obj' ~> env_obj)
-    a
-    (xs: (env_obj ~> a) * env_morphisms env_obj objs )
-    : (env_obj' ~> a) * env_morphisms env_obj' objs :=
-  match xs with
-  | pair x xs => pair (f >>> x) (map xs)
-  end.
-
-  (* Map over the environment object *)
-  Definition contra_map_morphisms
-    (env_obj env_obj': object)
-    (objs: list object)
-    (morphs: env_morphisms env_obj objs)
-    (f: env_obj' ~> env_obj)
-    : env_morphisms env_obj' objs.
-  Proof.
-    induction objs.
-    - exact tt.
-    - simpl in *. auto.
-      apply (contravariant_map' env_obj env_obj' objs IHobjs f).
-      auto.
-  Defined.
-
-  (* Build the morphisms of an evnironment by using the arrow methods 'exl' and
-  'exr' to extract eachs morphisms associated object from the environment object. *)
-  Definition build_morphisms (n: nat) (env: environment n):
-    env_morphisms (environment_as_object env) (environment_objects_as_list env).
-  Proof.
-    induction env; simpl.
-
-    - apply (contra_map_morphisms
-      (environment_as_object env)
-      (environment_as_object (ECons o env))
-      (environment_objects_as_list env )
-      ) in IHenv.
-      * intros.
-        exact (pair exl IHenv).
-      * exact exr.
-    - exact tt.
-  Defined.
-
-  Lemma env_length_is_n  (n: nat) (env: environment n):
-    length (environment_objects_as_list env) = n.
-  Proof.
-    induction env; simpl; auto.
-  Defined.
+  (****************************************************************************)
+  (* Environment lemmas                                                       *)
+  (****************************************************************************)
 
   Lemma lookup_bound:
     forall n o objs,
     lookup_object n objs = Some o
     -> n < length objs.
   Proof.
-    induction objs; intros.
+    induction objs; auto.
+  Qed.
 
-    - inversion H.
+  Hint Extern 3 =>
+    match goal with 
+    | [H: lookup_object _ _ = Some _|- _] => apply lookup_bound in H as H1
+    end : core.
 
-    - simpl in H.
-      destruct (Nat.eq_dec n (length objs)) as [n_eq | n_neq]; subst; auto.
-
-      rewrite H in IHobjs.
-      assert (Some o = Some o ).
-      auto.
-      apply IHobjs in H0.
-      simpl.
-      auto.
-  Defined.
-
-  Lemma lookup_bound_contra : forall o objs,
-    lookup_object (length objs) objs = Some o
-    -> False.
+  Lemma lookup_lower_contra : forall o n,
+    lookup_object n [] = Some o -> False.
   Proof.
-    intros.
-    apply lookup_bound in H.
-    apply Nat.lt_irrefl in H.
-    inversion H.
+    auto.
+  Qed.
+
+  Lemma lookup_upper_contra : forall o objs,
+    lookup_object (length objs) objs = Some o -> False.
+  Proof.
+    auto. 
+  Qed.
+
+  Hint Extern 1 => 
+    match goal with
+    | [H: lookup_object (length ?X) (?X) = Some _ |- _] => apply lookup_upper_contra in H; contradiction
+    | [H: lookup_object ?X [] = Some _ |- _] => apply lookup_lower_contra in H; contradiction
+    end : core.
+
+  (* Shorthand for passing evidence that a lookup is well formed *)
+  Notation ok_lookup := (
+    fun (n: nat) (env: list object) (o: object) => lookup_object n env = Some o
+  ).
+
+  (* Proof that looking up a morphism is the morphism from the environment to
+    * the object at the same index.
+    *)
+  Lemma ok_lookup_sets_lookup_morphism_ty : forall n o objs env_obj,
+    lookup_object n objs = Some o
+    -> lookup_morphism_ty n env_obj objs = morphism env_obj o.
+  Proof.
+    induction objs; auto.
   Defined.
 
-  Lemma push_lookup: forall n objs o a,
-    n < length objs
-    -> lookup_object n (a::objs) = Some o
-    -> lookup_object n objs = Some o.
+  Hint Immediate ok_lookup_sets_lookup_morphism_ty : core.
+
+  Lemma morphism_coerce:
+    forall (n:nat) env_obj o (objs: list object),
+    ok_lookup n objs o ->
+    lookup_morphism_ty n env_obj objs = morphism env_obj o.
   Proof.
-    intros.
-    case_eq (Nat.eq_dec n (length (objs))); intros.
-    - rewrite e in H.
-      apply Nat.lt_irrefl in H.
-      contradiction.
-    - simpl in H0.
-      rewrite H1 in H0.
-      apply H0.
-  Defined.
+    auto.
+  Qed.
+
+  Lemma environment_objects_length_is_n  (n: nat) (env: environment n):
+    length (as_object_list env) = n.
+  Proof.
+    induction env; auto.
+  Qed.
+
+  Hint Extern 4 => 
+    match goal with
+    | [H: context[length(as_object_list ?X)] |- _] => rewrite environment_objects_length_is_n in H
+    end : core.
 
   Lemma split_lookup : forall n env v1 y o,
-    (v1 = n /\ y = o) \/ lookup_object v1 (environment_objects_as_list env) = Some o
-    -> lookup_object v1 (environment_objects_as_list (@ECons n y env)) = Some o.
+    (n = v1 /\ y = o) \/ lookup_object v1 (as_object_list env) = Some o
+    -> lookup_object v1 (as_object_list (@ECons n y env)) = Some o.
   Proof.
-    intros.
-    simpl.
-    destruct (Nat.eq_dec v1 (length (environment_objects_as_list env))) as [n_eq | n_neq].
-    - inversion H.
-      * inversion H0.
-        f_equal. auto.
-      * rewrite n_eq in H0.
-        apply lookup_bound_contra in H0.
-        contradiction.
-    - inversion H; auto.
-      * inversion H0.
-        rewrite H1 in n_neq.
-        rewrite env_length_is_n in n_neq.
-        destruct n_neq.
-        auto.
+    auto 6.
+  Qed.
+
+  Lemma lookup_top_is_extraction: forall n m o o' env x, 
+    m = n
+    -> lookup_object m (as_object_list (@ECons n o env)) = Some o' 
+    -> morphism (o**x) o'.
+  Proof.
+    Hint Extern 1 => exact exl : core.
+    auto.
   Defined.
 
+  Lemma push_lookup : forall n env o o' x ,
+    x <> n ->
+    lookup_object x (as_object_list (@ECons n o' env)) = Some o ->
+    lookup_object x (as_object_list env) = Some o.
+  Proof.
+    Hint Extern 1 => lia : core.
+    auto.
+  Qed.
+
+  Fixpoint extract_nth n (env: environment n) o x
+    : (lookup_object x (as_object_list env) = Some o) -> morphism (as_object env) o :=
+  match env return
+    (lookup_object x (as_object_list env) = Some o) -> morphism (as_object env) o
+    with
+  | ENil => fun H => match lookup_lower_contra H with end
+  | @ECons n' o' env' => fun H =>
+    match eq_nat_dec x n' with
+    | left Heq => (lookup_top_is_extraction  _ env' _ Heq H)
+    | right Hneq =>  exr >>> extract_nth env' x (push_lookup _ _ Hneq H)
+    end
+  end.
+  
   (****************************************************************************)
   (* Closure conversion via de Brujin indices form                            *)
   (****************************************************************************)
-
   (* In de Brujin indexing variables are nats *)
+
   Definition natvar : object -> object -> Type := fun _ _ => nat.
 
   (* Reverse de Brujin indexing is well formed *)
@@ -250,12 +204,23 @@ Section WithArrow.
     (expr: kappa natvar i o) {struct expr}
     : Prop :=
   match expr with
-  | DVar x            => ok_lookup x (environment_objects_as_list env) o
+  | DVar x            => ok_lookup x (as_object_list env) o
   | @DAbs _ _ x y z f => wf_debrujin (@ECons n x env) (f n)
   | DApp e1 e2        => wf_debrujin env e1 /\ wf_debrujin env e2
   | DCompose e1 e2    => wf_debrujin env e1 /\ wf_debrujin env e2
   | DArr _            => True
   end.
+
+  Lemma wf_debrujin_succ: 
+    forall ix iy o 
+    (n: nat) (env: environment n)
+    (expr: kappa natvar (ix**iy) o)
+    f,
+    expr = DAbs f ->
+    @wf_debrujin (ix**iy) o n env expr -> @wf_debrujin iy o (S n) (ECons ix env) (f n).
+  Proof.
+    auto.
+  Qed.
 
   (* Perform closure conversion by passing an explicit environment. The higher
   order PHOAS representation is converted to first order form with de Brujin
@@ -269,20 +234,21 @@ Section WithArrow.
   *)
   Fixpoint closure_conversion {i o}
     (n: nat) (env: environment n)
-    (morphs: env_morphisms (environment_as_object env) (environment_objects_as_list env))
+    (* (morphs: env_morphisms (as_object env) (as_object_list env)) *)
     (expr: kappa natvar i o) {struct expr}
-    : wf_debrujin env expr -> morphism (i ** environment_as_object env) o :=
+    : wf_debrujin env expr -> morphism (i ** as_object env) o :=
   match expr with
     (* Instantiating a variable is done by 'exr' to select the environment, and
     then indexing using lookup_morphism. 'morphisms_coerce' and 'wf' are used to
     align the types and to prove to Coq that the lookup is well formed. *)
-  | DVar v => fun wf => exr >>> morphism_coerce _ wf (lookup_morphism (environment_as_object env) (environment_objects_as_list env) v morphs)
+  (* | DVar v => fun wf => exr >>> @extract_variable v n env (as_object env) _ (as_object_list env) (build_morphisms env) eq_refl eq_refl wf *)
+  | DVar v => fun wf => exr >>> extract_nth env v wf
     (* Kappa abstraction requires extending the environment which includes
     modifying all the variable morphisms in scope (and their types!).
     *)
-  | @DAbs _ _ x y z f => fun wf =>
+  | @DAbs _ _ x y _ f => fun wf =>
     let env' := ECons x env in
-    let f' := closure_conversion env' (build_morphisms env') (f n) wf in
+    let f' := closure_conversion env'  (f n) (wf_debrujin_succ _ eq_refl wf) in
     (* This line moves the first arrow argument into the right hand position,
     which allows 'assoc' to move the argument to the front of the environment
     f: x*y ~> o
@@ -300,9 +266,9 @@ Section WithArrow.
   *)
   | DApp f e => fun wf =>
     second (copy >>> first (uncancell
-    >>> closure_conversion env morphs e (proj2 wf)))
+    >>> closure_conversion env e (proj2 wf)))
     >>> unassoc >>> first swap
-    >>> closure_conversion env morphs f (proj1 wf)
+    >>> closure_conversion env f (proj1 wf)
 
     (* Alternatively *)
     (* copy *)
@@ -316,8 +282,8 @@ Section WithArrow.
   | DCompose e1 e2 => fun wf =>
     second copy
     >>> unassoc
-    >>> first (closure_conversion env morphs e2 (proj2 wf))
-    >>> closure_conversion env morphs e1 (proj1 wf)
+    >>> first (closure_conversion env e2 (proj2 wf))
+    >>> closure_conversion env e1 (proj1 wf)
 
   | DArr m => fun _ => exl >>> m
   end.
@@ -337,12 +303,12 @@ Section WithArrow.
       forall i o, ctxt
       -> kappa var1 i o -> kappa var2 i o
       -> Prop :=
-    | Var_equiv : forall x y v1 v2 E,
-      In (vars (obj_pair x y) (v1,v2)) E
-      -> kappa_equivalence E (DVar v1) (DVar v2)
+    | Var_equiv : forall i o n1 n2 E,
+      In (vars (obj_pair i o) (n1,n2)) E
+      -> kappa_equivalence E (DVar n1) (DVar n2)
 
-    | Abs_equiv : forall y (f1: var1 unit y -> kappa var1 unit y) f2 (E:ctxt),
-      (forall v1 v2, kappa_equivalence (vars (obj_pair unit y) (v1,v2) :: E) (f1 v1) (f2 v2))
+    | Abs_equiv : forall o (f1: var1 unit o -> kappa var1 unit o) f2 (E:ctxt),
+      (forall n1 n2, kappa_equivalence (vars (obj_pair unit o) (n1,n2) :: E) (f1 n1) (f2 n2))
       -> kappa_equivalence E (DAbs f1) (DAbs f2)
 
     | App_equiv : forall E x y z (f1 : kappa var1 (x**y) z) f2 e1 e2,
@@ -361,68 +327,57 @@ Section WithArrow.
   Axiom Kappa_equivalence : forall {i o} (expr: forall var, kappa var i o) var1 var2,
     kappa_equivalence nil (expr var1) (expr var2).
 
-  (* Recovering a dependent value requires gentle proof steps (?) to prevent the
-  equality disappearing. *)
-  Lemma recover_dependent_val: forall y n xi o v1 v2,
-    vars natvar natvar (obj_pair unit y) (n, n) = vars natvar natvar (obj_pair xi o) (v1, v2)
-    -> n = v1.
+  Notation variable_pair i o n1 n2 := (vars natvar natvar (obj_pair i o) (n1, n2)).
+
+  (* Evidence of variable pair equality *)
+  Notation match_pairs xo xn yi yo yn1 yn2 := 
+    (variable_pair unit xo xn xn = variable_pair yi yo yn1 yn2).
+
+  (* Evidence that if a given variable is in an environment we can lookup_object the object at the index. *)
+  Notation ok_variable_lookup := (fun env E =>
+    forall (i o : object) (n1 n2 : natvar i o),
+      In (vars natvar natvar (obj_pair i o) (n1, n2)) E
+      -> lookup_object n1 (as_object_list env) = Some o
+  ).
+
+  (* Recovering a dependent value requires recovering the type equality first to prevent the
+  value equality disappearing. *)
+  Lemma recover_dependent_val: forall xo xn yi yo yn1 yn2,
+    match_pairs xo xn yi yo yn1 yn2 -> (xn = yn1 /\ xo = yo).
   Proof.
     intros.
     inversion H.
     subst.
-    generalize (inj_pairT2 _ _ _ _ _ H).
+    generalize (inj_pairT2 _ _ _ _ _ H). 
     intro.
     inversion H0.
     auto.
-  Defined.
+  Qed.
 
-  Lemma found_at: forall n (env: environment n) v1 v2 o y xi,
-    vars natvar natvar (obj_pair unit y) (n, n) = vars natvar natvar (obj_pair xi o) (v1, v2)
-    -> (v1 = n /\ y = o).
+  Lemma apply_lookup : forall n (env: environment n) i o n1 n2 E,
+    In (variable_pair i o n1 n2) E
+    -> ok_variable_lookup env E
+    -> lookup_object n1 (as_object_list env) = Some o.
   Proof.
-    intros.
-    split.
-    apply recover_dependent_val in H.
+    Hint Extern 1 => 
+      match goal with
+      | [H1: In _ ?X, H2: ok_variable_lookup _ ?X |- _] => apply H2 in H1
+      end : core.
     auto.
-    inversion H.
-    auto.
-  Defined.
-
-  (* Evidence that a variable is in an environment at an index implies a given
-  object at a lookup_object index. *)
-  Notation lookup_in_vars := (fun env E =>
-    forall (xi xo : object) (v1 v2 : natvar xi xo),
-      In (vars natvar natvar (obj_pair xi xo) (v1, v2)) E
-      -> lookup_object v1 (environment_objects_as_list env) = Some xo
-  ).
-
-  Lemma lookup_in_extended_environment': forall n (env: environment n) v1 v2 xi xo y E,
-    lookup_in_vars env E
-    -> vars natvar natvar (obj_pair unit y) (n, n) = vars natvar natvar (obj_pair xi xo) (v1, v2) \/ lookup_object v1 (environment_objects_as_list env) = Some xo
-    -> lookup_object v1 (environment_objects_as_list (ECons y env)) = Some xo.
+  Qed.
+    
+  Lemma apply_extended_lookup: forall n env v1 v2 y i o E,
+    match_pairs y n i o v1 v2 \/ In (vars natvar natvar (obj_pair i o) (v1, v2)) E
+    -> ok_variable_lookup env E
+    -> lookup_object v1 (as_object_list (@ECons n y env)) = Some o.
   Proof.
-    intros.
-    rewrite split_lookup with (o:=xo); auto.
-    inversion H0.
-    - left.
-      apply found_at with (v2:=v2) (xi:=xi); auto.
-    - right.
-      apply H1.
-  Defined.
+    Hint Extern 3 => eapply recover_dependent_val : core.
+    Hint Resolve split_lookup : core.
+    eauto 7.
+  Qed.
 
-  Lemma lookup_in_extended_environment: forall n env v1 v2 y i o E,
-    lookup_in_vars env E
-    -> vars natvar natvar (obj_pair unit y) (n, n) = vars natvar natvar (obj_pair i o) (v1, v2) \/ In (vars natvar natvar (obj_pair i o) (v1, v2)) E
-    -> lookup_object v1 (environment_objects_as_list (@ECons n y env)) = Some o.
-  Proof.
-    intros.
-
-    eapply (lookup_in_extended_environment' H).
-
-    inversion H0.
-    - left. apply H1.
-    - right. apply H with (xi:=i) (v2:=v2). apply H1.
-  Defined.
+  Hint Immediate apply_lookup : core.
+  Hint Immediate apply_extended_lookup : core.
 
   (* Apply the auto generated kappa_equivalence_ind induction scheme rather than
   calling induction directly as calling induction directly results in too
@@ -430,35 +385,26 @@ Section WithArrow.
   Lemma kappa_wf
     : forall i o E (expr1 expr2: kappa natvar i o),
     kappa_equivalence E expr1 expr2
-    -> forall n (env: environment n), lookup_in_vars env E
+    -> forall n (env: environment n), ok_variable_lookup env E
     -> wf_debrujin env expr1.
-
+  Proof.
     apply (kappa_equivalence_ind
     (fun i o E (expr1 expr2 : kappa natvar i o) =>
       forall n (env: environment n),
-        (forall xi xo (v1 v2 : natvar xi xo), In (vars _ _ (obj_pair xi xo) (v1, v2)) E
-          -> lookup_object v1 (environment_objects_as_list env) = Some xo)
+        ok_variable_lookup env E
         -> wf_debrujin env expr1)
-        ); intros; simpl in *; auto.
+        ); eauto.
+  Qed.
 
-    - apply H0 in H. apply H.
-    - apply H0 with (v2:=n).
-      intros.
-      apply lookup_in_extended_environment with (env:=env) in H2.
-      apply H2.
-      auto.
-  Defined.
+  Hint Resolve kappa_wf : core.
+  Hint Resolve Kappa_equivalence : core.
 
   Theorem Kappa_wf: forall {i o} (expr: forall var, kappa var i o), @wf_debrujin _ _ 0 ENil (expr _).
   Proof.
-    intros.
-    eapply kappa_wf.
-    eapply Kappa_equivalence.
-    intros.
-    inversion H.
-  Defined.
+    eauto.
+  Qed.
 
 End WithArrow.
 
 Definition Closure_conversion {arr i o} (expr: @Kappa arr i o): i ~> o
-  := uncancelr >>> closure_conversion (ENil arr) tt (expr _) (Kappa_wf expr).
+  := uncancelr >>> closure_conversion (ENil arr) (expr _) (Kappa_wf expr).
